done

Foundation/Propositional/ClassicalSemantics/ZeroSubst.lean
@@ -6,10 +6,11 @@ variable {v : ClassicalSemantics.Valuation α} {φ ψ : Formula α}
 
 open Classical
 open Semantics (Valid)
+open Formula (atom)
 open Formula.ClassicalSemantics
 
 open Classical in
-noncomputable abbrev vfSubst (v : Valuation α) : ZeroSubstitution α := ⟨
+noncomputable def vfSubst (v : Valuation α) : ZeroSubstitution α := ⟨
     λ a => if v a then ⊤ else ⊥,
     by intro a; simp [Formula.subst.subst_atom]; split <;> tauto;
 ⟩
@@ -25,11 +26,79 @@ theorem exists_neg_zeroSubst_of_not_isTautology (h : ¬φ.isTautology)
   apply eq_fml_of_eq_atom (v := v) ?_ |>.not.mp
   . exact hv;
   . intro a;
-    simp [val];
+    simp [val, vfSubst];
     split <;> tauto;
 
 lemma isTautology_of_forall_zeroSubst : (∀ s : ZeroSubstitution α, ¬(∼(φ⟦s.1⟧)).isTautology) → φ.isTautology := by
   contrapose!;
   apply exists_neg_zeroSubst_of_not_isTautology;
+
+set_option push_neg.use_distrib true in
+lemma isTautology_vfSubst : v ⊧ φ ↔ (φ⟦(vfSubst v).1⟧.isTautology) := by
+  simp only [Formula.isTautology, Valid, Formula.subst.subst_atom, not_forall];
+  induction φ with
+  | hatom a =>
+    dsimp [vfSubst];
+    constructor;
+    . intro h w;
+      split;
+      . tauto;
+      . contradiction;
+    . intro h;
+      have := h v;
+      split at this;
+      . assumption;
+      . tauto;
+  | hfalsum => simp;
+  | himp φ ψ ihφ ihψ =>
+    constructor;
+    . intro h w hφ;
+      apply ihψ.mp;
+      apply h;
+      apply ihφ.mpr;
+      intro u;
+      apply equiv_of_letterless ?_ u w |>.mpr hφ;
+      exact φ.letterless_zeroSubst;
+    . intro h hφ;
+      apply ihψ.mpr;
+      intro w;
+      apply equiv_of_letterless ?_ v w |>.mp;
+      . apply h;
+        apply ihφ.mp hφ;
+      exact ψ.letterless_zeroSubst;
+  | hor φ ψ ihφ ihψ =>
+    constructor;
+    . rintro (h | h) w;
+      . left; apply ihφ.mp; assumption;
+      . right; apply ihψ.mp; assumption;
+    . intro h;
+      rcases h v with hφ | hψ;
+      . left;
+        apply ihφ.mpr;
+        intro w;
+        apply equiv_of_letterless ?_ v w |>.mp hφ;
+        exact φ.letterless_zeroSubst;
+      . right;
+        apply ihψ.mpr;
+        intro w;
+        apply equiv_of_letterless ?_ v w |>.mp hψ;
+        exact ψ.letterless_zeroSubst;
+  | hand φ ψ ihφ ihψ =>
+    constructor;
+    . rintro ⟨hφ, hψ⟩ w;
+      constructor;
+      . apply ihφ.mp hφ;
+      . apply ihψ.mp hψ;
+    . intro h;
+      have := h v;
+      constructor;
+      . apply ihφ.mpr;
+        intro w;
+        apply equiv_of_letterless ?_ v w |>.mp $ h v |>.1;
+        exact φ.letterless_zeroSubst;
+      . apply ihψ.mpr;
+        intro w;
+        apply equiv_of_letterless ?_ v w |>.mp $ h v |>.2;
+        exact ψ.letterless_zeroSubst;
 
 end LO.Propositional.ClassicalSemantics
